streaming encrypt

src/api/dotnet/Client.cs
@@ -8,6 +8,7 @@ using Dafny;
 using ibyteseq = Dafny.ISequence<byte>;
 using icharseq = Dafny.ISequence<char>;
 using encryptioncontext = Dafny.Map<Dafny.ISequence<byte>, Dafny.ISequence<byte>>;
+using EncryptionStreams;
 using Streams;
 using byteseq = Dafny.Sequence<byte>;
 using charseq = Dafny.Sequence<char>;
@@ -21,7 +22,7 @@ namespace AWSEncryptionSDK
         // TODO: Proper documentation
         // TODO: should return some custom stream that "reads" the encryption
         // ie it can't all be loaded into memory
-        public static OutputStream Encrypt(Stream plaintext, CMM cmm, Dictionary<string, string> encryptionContext = null, ushort? algorithmSuiteID = null, uint? frameLength = null) {
+        public static EncryptionStream Encrypt(Stream plaintext, CMM cmm, Dictionary<string, string> encryptionContext = null, ushort? algorithmSuiteID = null, uint? frameLength = null) {
             if (algorithmSuiteID != null && !AlgorithmSuite.__default.VALID__IDS.Elements.Contains((ushort)algorithmSuiteID)) {
                 throw new ArgumentException("Invalid algorithmSuiteID: " + algorithmSuiteID.ToString());
             }
@@ -34,14 +35,19 @@ namespace AWSEncryptionSDK
             var optAlgorithmSuiteID = algorithmSuiteID != null ? STL.Option<ushort>.create_Some((ushort)algorithmSuiteID) : STL.Option<ushort>.create_None();
             var optFrameLength = frameLength != null ? STL.Option<uint>.create_Some((uint)frameLength) : STL.Option<uint>.create_None();
             var dafnyEncryptionContext = encryptionContext != null ? STL.Option<encryptioncontext>.create_Some(ToDafnyEncryptionContext(encryptionContext)) : STL.Option<encryptioncontext>.create_None();
-            STL.Result<ESDKClient.EncryptorStream> result = ESDKClient.__default.StreamEncrypt(
+            
+            // THese two shuould be encapsulated by one object in dafny
+            STL.Result<ESDKClient.EncryptTheRestStream> result = ESDKClient.__default.StreamEncrypt(
                     dafnyStream,
                     cmm,
                     dafnyEncryptionContext,
                     optAlgorithmSuiteID,
                     optFrameLength
                     );
-            return new OutputStream(DafnyFFI.ExtractResult(result));
+            ESDKClient.EncryptInputStream input = new ESDKClient.EncryptInputStream();
+            input.__ctor(dafnyStream);
+
+            return new EncryptionStream(input, DafnyFFI.ExtractResult(result));
         }
   
         // TODO: Proper documentation
@@ -49,7 +55,6 @@ namespace AWSEncryptionSDK
         // ie it can't all be loaded into memory
         public static MemoryStream Decrypt(Stream cyphertext, CMM cmm) {
             ibyteseq dafnyPlaintext = DafnyFFI.SequenceFromStream(cyphertext);
-    
             // TODO: Might need a lock here if ANYTHING in the Dafny runtime isn't threadsafe!
             STL.Result<ibyteseq> result = ESDKClient.__default.Decrypt(dafnyPlaintext, cmm);
     
