src/api/dotnet/EncryptionStream.cs
@@ -1,0 +1,113 @@
+using System;
+using System.IO;
+using ESDKClient;
+using STL;
+
+// TODO I can't name this EncryptionStream :'(
+namespace EncryptionStreams {
+    // What's used internally and exposes externally should be different... Right now the C# interface
+    // is used for both
+    // TODO implement Disposable, wrap stream in friendly handlers
+    public partial class EncryptionStream : Stream {
+        // TODO what should the underlying stream actually be?
+        // TODO should be readonly
+        private ESDKClient.EncryptTheRestStream encryptorStream;
+        private ESDKClient.EncryptInputStream inputStream;
+
+        public EncryptionStream(ESDKClient.EncryptInputStream inputStream, ESDKClient.EncryptTheRestStream encryptorStream) {
+            this.inputStream = inputStream;
+            this.encryptorStream = encryptorStream;
+        }
+
+        public override bool CanRead
+        {
+            get
+            {
+                return true;
+            }
+        }
+
+        public override bool CanSeek
+        {
+            get
+            {
+                return false;
+            }
+        }
+
+        public override bool CanWrite
+        {
+            get
+            {
+                return false;
+            }
+        }
+
+        public override void Flush()
+        {
+          // Do nothing. Docs say to do this instead of throw because it should be valid to flush a readonly stream
+        }
+
+        public override long Length
+        {
+            get
+            {
+                throw new NotSupportedException();
+            }
+        }
+
+        public override long Position
+        {
+            get
+            {
+                throw new NotSupportedException();
+            }
+            set
+            {
+                throw new NotSupportedException();
+            }
+        }
+
+        public override int Read(byte[] buffer, int offset, int count)
+        {
+            int n = 0;
+            // FIXME currently initializing buffer fo revery read. obvi fix this
+            // also naming collision
+
+            // Need to abstract more so that we do not have to byte by byte HasNext()
+            while (n < count) {
+                while (!encryptorStream.HasNext()) {
+                    // TODO annoying BigInteger >:(
+                    System.Numerics.BigInteger siphoned = DafnyFFI.ExtractResult(inputStream.Siphon(encryptorStream));
+                    // there is no more to siphon. End of composite stream.
+                    if (siphoned == 0) {
+                        return n;
+                    }
+                    // assert HasNext()?
+                }
+                byte readByte = DafnyFFI.ExtractResult(encryptorStream.Next());
+
+                // TODO 0 could be a failure or EOF, which is unfortunate.
+                // For now just read it as is. Implement proper failures later.
+                buffer[offset+n] = readByte;
+                n += 1;
+            }
+            return n;
+        }
+
+        public override long Seek(long offset, SeekOrigin origin)
+        {
+            throw new NotSupportedException();
+        }
+
+        public override void SetLength(long value)
+        {
+            throw new NotSupportedException();
+        }
+
+        public override void Write(byte[] buffer, int offset, int count)
+        {
+            throw new NotSupportedException();
+        }
+    }
+}
