src/SDK/Client.dfy
@@ -34,217 +34,73 @@ module {:extern "ESDKClient"} ESDKClient {
 
   const DEFAULT_FRAME_LENGTH: uint32 := 4096
 
-  class EncryptorStream extends Collections.ByteProducer {
-    // TODO having issues with extern constructors
-    //constructor(bytes: seq<uint8>) {}
-    // The top level one shouldn't actually have to deal with internal buffers
+  // This is just a transformation of the C# stream interface with the Dafny producer interface
+  // TODO move this encapsulation into the api/extern layer
+  class EncryptInputStream extends Collections.ByteProducer {
     var inStream: Streams.InputStream
-    var index: int
-    // TODO have to declare here if we want verification around it. Brittle.
-    var cmm: CMMDefs.CMM
-    var optEncryptionContext: Option<Materials.EncryptionContext>
-    var algorithmSuiteID: Option<AlgorithmSuite.ID>
-    var optFrameLength: Option<uint32>
-    var length: int32
-    var downStream: MessageHeaderStream
 
     predicate Valid() reads this ensures Valid() ==> this in Repr {
-      // TODO check downstream is valid?
       && this in Repr
     }
 
-    constructor(inStream: Streams.InputStream, cmm: CMMDefs.CMM, optEncryptionContext: Option<Materials.EncryptionContext>, algorithmSuiteID: Option<AlgorithmSuite.ID>, optFrameLength: Option<uint32>)
+    constructor(inStream: Streams.InputStream)
       ensures fresh(Repr - {this})
     {
-      // TODO most all of this stuff is just needed to pass down to MessageHeaderStream.
-      // It would be better to create that outside this and compose them together?
-      // Or should this be responsible for creating and composing all sub streams?
       this.Repr := {this};
       this.inStream := inStream;
-      this.cmm := cmm;
-      this.optEncryptionContext := optEncryptionContext;
-      this.algorithmSuiteID := algorithmSuiteID;
-      this.optFrameLength := optFrameLength;
-      this.downStream := new MessageHeaderStream(inStream, cmm, optEncryptionContext, algorithmSuiteID, optFrameLength);
     }
 
-    // TODO Not sure how this should fit together...
-    method HasNext() returns (b: bool)
+    predicate method HasNext()
       requires Valid()
       ensures Valid()
     {
-      b := downStream.HasNext();
-    }
-
-    method Next() returns (res: Result<uint8>) 
-      requires Valid()
-      //requires HasNext()
-      ensures Valid()
-      modifies this
-    {
-      // TODO This is brittle, HasNext can't guarantee that this will succeed,
-      // especially since we might experience a failure in a transformation done
-      // in the downstream. Right now failures and EOF are propogating up as 0.
-      res := downStream.Next();
-    }
-
-    method Siphon(consumer: Collections.ByteConsumer) returns (siphoned: Result<int>) 
-      requires Valid()
-      requires consumer.Valid()
-      requires this !in consumer.Repr
-      requires consumer !in Repr
-      requires Repr !! consumer.Repr
-      ensures Valid()
-      modifies this, Repr, consumer, consumer.Repr
-      decreases *
-    {
-      // Use default siphon. Is there a subtype check we could be making here
-      // to improve performance in certain cases?
-      siphoned := Collections.DefaultSiphon(this, consumer);
-    }
-  }
-
-  class MessageHeaderStream extends Collections.ByteProducer {
-    // TODO having issues with extern constructors
-    //constructor(bytes: seq<uint8>) {}
-    var inStream: Streams.InputStream
-    var inBuffer: seq<uint8> // Use the byteReader/Writer?
-    var outBuffer: seq<uint8>
-    var cmm: CMMDefs.CMM
-    var optEncryptionContext: Option<Materials.EncryptionContext>
-    var algorithmSuiteID: Option<AlgorithmSuite.ID>
-    var optFrameLength: Option<uint32>
-    var length: int32
-    var didTheThing: bool
-    var downStream: EncryptTheRestStream
-
-    predicate Valid() reads this ensures Valid() ==> this in Repr {
-      // TODO check downstream Valid?
-      && this in Repr
-    }
-
-    constructor(inStream: Streams.InputStream, cmm: CMMDefs.CMM, optEncryptionContext: Option<Materials.EncryptionContext>, algorithmSuiteID: Option<AlgorithmSuite.ID>, optFrameLength: Option<uint32>) {
-      this.inStream := inStream;
-      this.cmm := cmm;
-      this.optEncryptionContext := optEncryptionContext;
-      this.algorithmSuiteID := algorithmSuiteID;
-      this.optFrameLength := optFrameLength;
-      this.inBuffer := [];
-      this.outBuffer := [];
-      this.didTheThing := false;
-      this.downStream := new EncryptTheRestStream(inStream, cmm, optEncryptionContext, algorithmSuiteID, optFrameLength);
-    }
-
-    // TODO Not sure how this should fit together...
-    method HasNext() returns (b: bool)
-      requires Valid()
-      ensures Valid()
-    {
-      b := downStream.HasNext();
-    }
-
-    method Next() returns (res: Result<uint8>) 
-      requires Valid()
-      //requires HasNext()
-      ensures Valid()
-      modifies this
-    {
-      // serialize the message header with our info on first read.
-      if !didTheThing {
-        var _ :- FillOutBuffer();
-        // we did the thing, so flip the bool so we don't do it again.
-        didTheThing := true;
-        expect |outBuffer| > 0;
-      }
-      // if we have stuff in the outBuffer. Take from that.
-      if |outBuffer| > 0 {
-        var byte := outBuffer[0];
-        // TODO will this grab correctly in the case that |outBuffer| == 1?
-        outBuffer := outBuffer[1..];
-        return Success(byte);
-      }
-      // if we don't have anything in the outBuffer and we did the thing, then
-      // that means we need to send to the next streaming interface in order
-      // to deal with the actual encryption
-      res := downStream.Next();
-    }
-
-    method Siphon(consumer: Collections.ByteConsumer) returns (siphoned: Result<int>) 
-      requires Valid()
-      requires consumer.Valid()
-      requires this !in consumer.Repr
-      requires consumer !in Repr
-      requires Repr !! consumer.Repr
-      ensures Valid()
-      modifies this, Repr, consumer, consumer.Repr
-      decreases *
-    {
-      // Use default siphon. Is there a subtype check we could be making here
-      // to improve performance in certain cases?
-      siphoned := Collections.DefaultSiphon(this, consumer);
-    }
-
-    // We don't actually have to read anything from the input stream
-    // in order to make the header.
-    // Call this the first time the stream is read.
-    // TODO make this foolproof
-    // TODO remove Result<bool> :P
-    method FillOutBuffer() returns (res: Result<bool>) {
-      var encryptionContext := optEncryptionContext.GetOrElse(map[]);
-      assert Msg.ValidAAD(encryptionContext) by {
-        reveal Msg.ValidAAD();
-        assert Msg.ValidAAD(encryptionContext);
-      }
-      var frameLength := if optFrameLength.Some? then optFrameLength.get else DEFAULT_FRAME_LENGTH;
-      
-      // This assumes inStream is seekable :/
+      // :'(
+      var pos := inStream.Position();
       var len := inStream.Length();
-      var encMatRequest := Materials.EncryptionMaterialsRequest(encryptionContext, algorithmSuiteID, Some(len as nat));
-      var encMat :- cmm.GetEncryptionMaterials(encMatRequest);
-      if UINT16_LIMIT <= |encMat.encryptedDataKeys| {
-        return Failure("Number of EDKs exceeds the allowed maximum.");
+      pos != len
+    }
+
+    method Next() returns (res: Result<uint8>) 
+      requires Valid()
+      requires HasNext()
+      ensures Valid()
+      modifies this
+    {
+      var buffer: seq<uint8> := seq(1, _ => 0);
+      // This is assuming inStream is a C# streaming interface
+      // As stated above, the transformation between C# and Dafny streaming interfaces
+      // must exist in the extern/api layer
+      // TODO This is brittle, and we don't even have HasNext guarantee anymore
+      var n := inStream.Read(buffer, 0, 1);
+      if n == 0 {
+        return Failure("Tried to read from input stream when nothing there");
       }
+      // This MUST be true or the API contract has been broken
+      expect n == 1;
+      return Success(buffer[0]);
+    }
 
-      var messageID: Msg.MessageID :- Random.GenerateBytes(Msg.MESSAGE_ID_LEN as int32);
-      var derivedDataKey := DeriveKey(encMat.plaintextDataKey.get, encMat.algorithmSuiteID, messageID);
-  
-      // Assemble and serialize the header and its authentication tag
-      var headerBody := Msg.HeaderBody(
-        Msg.VERSION_1,
-        Msg.TYPE_CUSTOMER_AED,
-        encMat.algorithmSuiteID,
-        messageID,
-        encMat.encryptionContext,
-        Msg.EncryptedDataKeys(encMat.encryptedDataKeys),
-        Msg.ContentType.Framed,
-        encMat.algorithmSuiteID.IVLength() as uint8,
-        frameLength);
-      var wr := new Streams.ByteWriter();
-
-      var _ :- Serialize.SerializeHeaderBody(wr, headerBody);
-      var unauthenticatedHeader := wr.GetDataWritten();
-
-      var iv: seq<uint8> := seq(encMat.algorithmSuiteID.IVLength(), _ => 0);
-      var encryptionOutput :- AESEncryption.AESEncrypt(encMat.algorithmSuiteID.EncryptionSuite(), iv, derivedDataKey, [], unauthenticatedHeader);
-      var headerAuthentication := Msg.HeaderAuthentication(iv, encryptionOutput.authTag);
-      var _ :- Serialize.SerializeHeaderAuthentication(wr, headerAuthentication, encMat.algorithmSuiteID);
-      outBuffer := wr.GetDataWritten();
-
-      // TODO better way to do this
-      downStream.SetDerivedValues(outBuffer, headerBody, derivedDataKey, encMat);
-      return Success(true);
+    method Siphon(consumer: Collections.ByteConsumer) returns (siphoned: Result<int>) 
+      requires Valid()
+      requires consumer.Valid()
+      requires this !in consumer.Repr2
+      requires consumer !in Repr
+      requires Repr !! consumer.Repr2
+      ensures Valid()
+      modifies this, Repr, consumer, consumer.Repr2
+      decreases *
+    {
+      // Use default siphon. Is there a subtype check we could be making here
+      // to improve performance in certain cases?
+      siphoned := Collections.DefaultSiphon(this, consumer);
     }
   }
 
-  // For now this stream just fills the rest of the buffer with the input stream,
-  // then encrypts that plaintext.
-  // This should be broken into parts so that it is not necessary to fill then entire
-  // plaintext/ciphertext into memory. But right now we're focusing on the streaming
-  // interface.
-  class EncryptTheRestStream extends Collections.ByteProducer {
-    // TODO having issues with extern constructors
-    //constructor(bytes: seq<uint8>) {}
-    var inStream: Streams.InputStream
+  // passes through the header and encrypts the plaintext
+  // This will read all of the plaintext into memory before
+  // performing the encryption because this is a proof of concept
+  // for the streaming interface.
+  class EncryptTheRestStream extends Collections.ByteProducer, Collections.ByteConsumer {
     var inBuffer: seq<uint8> // Use the byteReader/Writer?
     var outBuffer: seq<uint8>
     var cmm: CMMDefs.CMM
@@ -256,6 +112,12 @@ module {:extern "ESDKClient"} ESDKClient {
     var header: Msg.HeaderBody
     var dataKey: seq<uint8>
     var encMat: Materials.EncryptionMaterials
+    var seqNum: uint32
+    var isFinalFrame: bool
+    var finished: bool
+    var totalLength: int
+    var curLength: int
+    var toSign: seq<uint8>
 
     predicate Valid() reads this ensures Valid() ==> this in Repr {
       // TODO check downstream Valid?
@@ -263,33 +125,90 @@ module {:extern "ESDKClient"} ESDKClient {
     }
 
     // more woof.
-    constructor(inStream: Streams.InputStream, cmm: CMMDefs.CMM, optEncryptionContext: Option<Materials.EncryptionContext>, algorithmSuiteID: Option<AlgorithmSuite.ID>, optFrameLength: Option<uint32>) {
-      this.inStream := inStream;
+    constructor(cmm: CMMDefs.CMM, optEncryptionContext: Option<Materials.EncryptionContext>, algorithmSuiteID: Option<AlgorithmSuite.ID>, optFrameLength: Option<uint32>, serHeader: seq<uint8>, header: Msg.HeaderBody, dataKey: seq<uint8>, encMat: Materials.EncryptionMaterials, totalLength: int) {
       this.cmm := cmm;
       this.optEncryptionContext := optEncryptionContext;
       this.algorithmSuiteID := algorithmSuiteID;
       this.optFrameLength := optFrameLength;
       this.inBuffer := [];
-      this.outBuffer := [];
-    }
-
-    method SetDerivedValues(serHeader: seq<uint8>, header: Msg.HeaderBody, dataKey: seq<uint8>, encMat: Materials.EncryptionMaterials)
-    {
+      this.outBuffer := serHeader;
       this.serHeader := serHeader;
       this.header := header;
       this.encMat := encMat;
       this.dataKey := dataKey;
+      this.seqNum := 1;
+      this.isFinalFrame := false;
+      this.finished := false;
+      this.totalLength := totalLength;
+      this.curLength := 0;
+      // TODO :(
+      this.toSign := serHeader;
     }
 
-    // TODO Better way to do this...
-    method HasNext() returns (b: bool)
+    predicate method CanAccept() reads this, Repr
       requires Valid()
       ensures Valid()
     {
-      // :'(
-      var pos := inStream.Position();
-      var len := inStream.Length();
-      return !(pos == len && |outBuffer| == 0);
+      !finished
+    }
+    
+    method Accept(b: uint8) returns (res: Result<()>)
+      requires Valid()
+      requires CanAccept()
+      ensures Valid()
+      modifies this, Repr
+    {
+      // Add to inBuffer
+
+      inBuffer := inBuffer + [b];
+
+      // TODO update total Length
+      curLength := curLength + 1;
+
+      var frameLength := header.frameLength;
+
+      // TODO This is the only way we can know when to encrypt the final frame right now :(
+      if totalLength == curLength {
+        var frameToProcess := inBuffer;
+        inBuffer := [];
+        var encryptedFrame :- MessageBody.EncryptFinalFrame(encMat.algorithmSuiteID, dataKey, frameLength as int, header.messageID, frameToProcess, seqNum);
+        finished := true;
+        outBuffer := outBuffer + encryptedFrame;
+        toSign := toSign + encryptedFrame;
+        var res :- AddSignatureToOutBuffer();
+      } else if |inBuffer| >= frameLength as int {
+        var frameToProcess := inBuffer[..frameLength];
+        inBuffer := inBuffer[frameLength..];
+        var encryptedFrame :- MessageBody.EncryptRegularFrame(encMat.algorithmSuiteID, dataKey, frameLength as int, header.messageID, frameToProcess, seqNum);
+        outBuffer := outBuffer + encryptedFrame;
+        toSign := toSign + encryptedFrame;
+      }
+      return Success(());
+    }
+
+    method AddSignatureToOutBuffer() returns (res: Result<bool>) {
+      match encMat.algorithmSuiteID.SignatureType() {
+        case None =>
+        return Success(true);
+          // don't use a footer
+        case Some(ecdsaParams) =>
+          var digest :- Signature.Digest(ecdsaParams, toSign);
+          var bytes :- Signature.Sign(ecdsaParams, encMat.signingKey.get, digest);
+          if |bytes| != ecdsaParams.SignatureLength() as int {
+            return Failure("Malformed response from Sign().");
+          }
+          outBuffer := outBuffer + UInt16ToSeq(|bytes| as uint16) + bytes;
+          return Success(true);
+      }
+    }
+
+    // TODO Better way to do this...
+    predicate method HasNext()
+      reads this
+      requires Valid()
+      ensures Valid()
+    {
+      |outBuffer| > 0
     }
 
     method Next() returns (res: Result<uint8>) 
@@ -305,72 +224,16 @@ module {:extern "ESDKClient"} ESDKClient {
         outBuffer := outBuffer[1..];
         return Success(byte);
       }
-      // Read from input stream until we get enough where we can output something
-      // (which right now means read everything :P)
-      var len := inStream.Length();
-      var bytesInput: seq<uint8> := seq(1, _ => 0);
-      while |inBuffer| < len as int {
-        // This is assuming inStream is a C# streaming interface
-        var n := inStream.Read(bytesInput, 0, 1);
-        // we've reached the end of the input stream! This shouldn't happen unless we were wrong
-        // about len :/
-        if n == 0 {
-          // This shouldn't happen because this method can only be called
-          // if inStream.Position != inStream.Length
-          // If it does anyway, :shrug: return 0.
-          // FIXME
-          return Success(0);
-        }
-        // If not 0 it MUST be 1
-        expect n == 1;
-        // TODO this way of adding byte by byte will be REALLY slow. But simpifying implementation
-        // for now by assuming that the streaming is byte by byte.
-        inBuffer := inBuffer + [bytesInput[0]];
-        // So we have some more input, but do we have enough so that we can output a byte?
-        // For now, we can't output anything until we input everything.
-        // If we've buffered everything into memory, do the whole encryption
-        // TODO Will we always know inStream's length? No, what do we do in that case?
-      }
-      // if we're going byte by byte this MUST be true
-      // we've loaded all the plaintext into the inBuffer
-      expect |inBuffer| == len as int;
-
-      // Time to do the actual encryption
-      // Encrypt the given plaintext into the message body and add a footer with a signature, if required
-      var body :- MessageBody.EncryptMessageBody(inBuffer, header.frameLength as int, header.messageID, dataKey, encMat.algorithmSuiteID);
-      var msg := serHeader + body;
-
-      match encMat.algorithmSuiteID.SignatureType() {
-        case None =>
-          // don't use a footer
-        case Some(ecdsaParams) =>
-          var digest :- Signature.Digest(ecdsaParams, msg);
-          var bytes :- Signature.Sign(ecdsaParams, encMat.signingKey.get, digest);
-          if |bytes| != ecdsaParams.SignatureLength() as int {
-            return Failure("Malformed response from Sign().");
-          }
-          // TODO this hurt you
-          body := body + UInt16ToSeq(|bytes| as uint16) + bytes;
-      }
-      // Grab the one byte we want to return
-      var byte := body[0];
-      // Add the rest to the buffer
-      // the outBuffer MUST be empty if we were reading from input
-      expect |outBuffer| == 0;
-      outBuffer := body[1..];
-      // consume the inputBuffer
-      inBuffer := [];
-      return Success(byte); 
     }
 
     method Siphon(consumer: Collections.ByteConsumer) returns (siphoned: Result<int>) 
       requires Valid()
       requires consumer.Valid()
-      requires this !in consumer.Repr
+      requires this !in consumer.Repr2
       requires consumer !in Repr
-      requires Repr !! consumer.Repr
+      requires Repr !! consumer.Repr2
       ensures Valid()
-      modifies this, Repr, consumer, consumer.Repr
+      modifies this, Repr, consumer, consumer.Repr2
       decreases *
     {
       // Use default siphon. Is there a subtype check we could be making here
@@ -379,17 +242,62 @@ module {:extern "ESDKClient"} ESDKClient {
     }
   }
 
-  method StreamEncrypt(inStream: Streams.InputStream, cmm: CMMDefs.CMM, optEncryptionContext: Option<Materials.EncryptionContext>, algorithmSuiteID: Option<AlgorithmSuite.ID>, optFrameLength: Option<uint32>) returns (res: Result<EncryptorStream>)
+  method StreamEncrypt(inStream: Streams.InputStream, cmm: CMMDefs.CMM, optEncryptionContext: Option<Materials.EncryptionContext>, algorithmSuiteID: Option<AlgorithmSuite.ID>, optFrameLength: Option<uint32>) returns (res: Result<EncryptTheRestStream>)
     requires cmm.Valid()
     requires optFrameLength.Some? ==> optFrameLength.get != 0
     requires optEncryptionContext.Some? ==> optEncryptionContext.get.Keys !! Materials.ReservedKeyValues && Msg.ValidAAD(optEncryptionContext.get)
     decreases *
   {
-    // This should be a composition of them, not some noop stream wrapping them in a stack
-    var outStream := new EncryptorStream(inStream, cmm, optEncryptionContext, algorithmSuiteID, optFrameLength);
-    //var _ := outStream.FillBuffer(ciphertext);
+    // create  header and related values
+    var encryptionContext := optEncryptionContext.GetOrElse(map[]);
+    assert Msg.ValidAAD(encryptionContext) by {
+      reveal Msg.ValidAAD();
+      assert Msg.ValidAAD(encryptionContext);
+    }
+    var frameLength := if optFrameLength.Some? then optFrameLength.get else DEFAULT_FRAME_LENGTH;
+      
+    // This assumes inStream is seekable :/
+    // Should return None if not seekable?
+    var len := inStream.Length();
+    var encMatRequest := Materials.EncryptionMaterialsRequest(encryptionContext, algorithmSuiteID, Some(len as nat));
+    var encMat :- cmm.GetEncryptionMaterials(encMatRequest);
+    if UINT16_LIMIT <= |encMat.encryptedDataKeys| {
+      return Failure("Number of EDKs exceeds the allowed maximum.");
+    }
 
-    return Success(outStream);
+    var messageID: Msg.MessageID :- Random.GenerateBytes(Msg.MESSAGE_ID_LEN as int32);
+    var derivedDataKey := DeriveKey(encMat.plaintextDataKey.get, encMat.algorithmSuiteID, messageID);
+
+    // Assemble and serialize the header and its authentication tag
+    var headerBody := Msg.HeaderBody(
+      Msg.VERSION_1,
+      Msg.TYPE_CUSTOMER_AED,
+      encMat.algorithmSuiteID,
+      messageID,
+      encMat.encryptionContext,
+      Msg.EncryptedDataKeys(encMat.encryptedDataKeys),
+      Msg.ContentType.Framed,
+      encMat.algorithmSuiteID.IVLength() as uint8,
+      frameLength);
+    var wr := new Streams.ByteWriter();
+
+    var _ :- Serialize.SerializeHeaderBody(wr, headerBody);
+    var unauthenticatedHeader := wr.GetDataWritten();
+
+    var iv: seq<uint8> := seq(encMat.algorithmSuiteID.IVLength(), _ => 0);
+    var encryptionOutput :- AESEncryption.AESEncrypt(encMat.algorithmSuiteID.EncryptionSuite(), iv, derivedDataKey, [], unauthenticatedHeader);
+    var headerAuthentication := Msg.HeaderAuthentication(iv, encryptionOutput.authTag);
+    var _ :- Serialize.SerializeHeaderAuthentication(wr, headerAuthentication, encMat.algorithmSuiteID);
+
+    var data := wr.GetDataWritten();
+    // This should be a composition of them, not some noop stream wrapping them in a stack
+    // Should have header be ingested into finalStream, right now just passing it to constructor :/
+    var finalStream := new EncryptTheRestStream(cmm, optEncryptionContext, algorithmSuiteID, optFrameLength, data, headerBody, derivedDataKey, encMat, len as int);
+    //var _ := outStream.FillBuffer(ciphertext);
+    
+    // TODO some way to have a "composed" stream
+
+    return Success(finalStream);
     // TODO convert to output stream
   }
 
